rustfrontend/Rustlightown.v
@@ -726,7 +726,6 @@ Fixpoint split_fully_own_place (p: place) (ty: type) :=
   | _ => nil
   end.
 
-
 (* Drop place state *)
 
 Inductive drop_place_state : Type :=
@@ -749,7 +748,16 @@ Definition gen_drop_place_state (p: place) : drop_place_state :=
           drop_fully_owned_box (p' :: l)
       end
   end.
-          
+
+Definition split_partial_own_place (p: place) :=
+  match typeof_place p with
+  | Tbox _ =>
+      [p]
+  | _ =>
+      []
+  end.
+
+
 (** Continuation *)
 
 
@@ -1378,7 +1386,7 @@ Inductive step_dropplace : state -> trace -> state -> Prop :=
       (Dropplace f None ps k le own m)
 | step_dropplace_init2: forall f p ps k le own m st (full: bool)
     (OWN: is_init own p = true)
-    (DPLACE: st = (if full then gen_drop_place_state p else drop_fully_owned_box [p])),
+    (DPLACE: st = (if full then gen_drop_place_state p else drop_fully_owned_box (split_partial_own_place p))),
     step_dropplace (Dropplace f None ((p, full) :: ps) k le own m) E0
       (Dropplace f (Some st) ps k le (move_place own p) m)
 | step_dropplace_box: forall le m m' k ty b' ofs' f b ofs p own ps l
